src/HOL/Quickcheck_Exhaustive.thy
@@ -142,9 +142,6 @@ instance ..
 
 end
 
-definition (in term_syntax) [code_unfold]: "valterm_emptyset = Code_Evaluation.valtermify ({} :: ('a :: typerep) set)"
-definition (in term_syntax) [code_unfold]: "valtermify_insert x s = Code_Evaluation.valtermify insert {\<cdot>} (x :: ('a :: typerep * _)) {\<cdot>} s"
-
 instantiation set :: (full_exhaustive) full_exhaustive
 begin
 
